concurrency/hack-hash-table/ResourceStateMachine_Refines_AsyncMapSpec.i.dfy
@@ -11,6 +11,8 @@ module ResourceStateMachine_Refines_AsyncMapSpec {
   import Multisets
   import MapSpec
   import Ifc = AsyncIfc
+  import MapIfc
+  import opened KeyValueType
 
   function req_of_ticket(t: HT.Ticket) : B.Req {
     B.Req(t.rid, t.input)
@@ -35,7 +37,8 @@ module ResourceStateMachine_Refines_AsyncMapSpec {
     B.Variables(
       MapSpec.Variables(map_remove_nones(t.ops)),
       reqs_of_tickets(s.tickets),
-      resps_of_stubs(t.stubs)
+      resps_of_stubs(s.stubs)
+          + resps_of_stubs(t.stubs)
           + resps_of_stubs(apply_to_query_stub(t.queries))
           + resps_of_stubs(apply_to_remove_stub(t.removes))
     )
@@ -47,6 +50,10 @@ module ResourceStateMachine_Refines_AsyncMapSpec {
     ensures A.Inv(s')
     ensures B.Next(I(s), I(s'), Ifc.InternalOp)
   {
+    MultisetLemmas.MultisetSimplificationTriggers<HT.Ticket, B.Req>();
+    MultisetLemmas.MultisetSimplificationTriggers<HT.Stub, B.Resp>();
+    MultisetLemmas.MultisetSimplificationTriggers<S.QueryRes, HT.Stub>();
+
     var step :| HT.UpdateStep(s, s', step);
     match step {
       case InsertSkipStep(pos) => {
@@ -57,6 +64,8 @@ module ResourceStateMachine_Refines_AsyncMapSpec {
       }
       case InsertDoneStep(pos) => {
         InsertDone_PreservesInterp(s, s', pos);
+        //assert I(s).resps == I(s').resps;
+        //assert I(s) == I(s');
       }
       case InsertUpdateStep(pos) => {
         InsertUpdate_PreservesInterp(s, s', pos);
@@ -75,6 +84,17 @@ module ResourceStateMachine_Refines_AsyncMapSpec {
       }
       case RemoveDoneStep(pos) => {
         RemoveDone_PreservesInterp(s, s', pos);
+
+        /*assert resps_of_stubs(s.stubs) + multiset{B.Resp(s.table[pos].value.state.rid, MapIfc.RemoveOutput(true))}
+            == resps_of_stubs(s'.stubs);
+        assert resps_of_stubs(apply_to_remove_stub(interp(s.table).removes))
+            == resps_of_stubs(apply_to_remove_stub(interp(s'.table).removes)) + multiset{B.Resp(s.table[pos].value.state.rid, MapIfc.RemoveOutput(true))};
+        assert resps_of_stubs(s.stubs)
+                + resps_of_stubs(apply_to_remove_stub(interp(s.table).removes))
+            == resps_of_stubs(s'.stubs)
+                + resps_of_stubs(apply_to_remove_stub(interp(s'.table).removes));
+        assert I(s).resps == I(s').resps;
+        assert I(s) == I(s');*/
       }
       case QuerySkipStep(pos) => {
         QuerySkip_PreservesInterp(s, s', pos);
@@ -88,13 +108,73 @@ module ResourceStateMachine_Refines_AsyncMapSpec {
 
       case ProcessInsertTicketStep(insert_ticket) => {
         ProcessInsertTicket_ChangesInterp(s, s', insert_ticket);
+        var I_s := I(s);
+        var I_s' := I(s');
+        var rid := insert_ticket.rid;
+        var input := insert_ticket.input;
+        var output := MapIfc.InsertOutput(true);
+
+        assert s.tickets == s'.tickets + multiset{insert_ticket};
+        /*assert resps_of_stubs(interp(s'.table).stubs)
+            == resps_of_stubs(interp(s.table).stubs) + multiset{B.Resp(rid, output)};
+        assert B.Req(rid, input) in I_s.reqs;
+        assert I_s.reqs == I_s'.reqs + multiset{B.Req(rid, input)};
+        assert I_s'.resps == I_s.resps + multiset{B.Resp(rid, output)};
+        assert MapSpec.Next(I_s.s, I_s'.s, MapIfc.Op(input, output));*/
+        assert B.LinearizationPoint(I_s, I_s', rid, input, output);
       }
       case ProcessRemoveTicketStep(remove_ticket) => {
         ProcessRemoveTicket_ChangesInterp(s, s', remove_ticket);
+        assert s.tickets == s'.tickets + multiset{remove_ticket};
+        assert B.LinearizationPoint(I(s), I(s'), remove_ticket.rid, remove_ticket.input,
+            MapIfc.RemoveOutput(remove_ticket.input.key in I(s).s.m));
       }
       case ProcessQueryTicketStep(query_ticket) => {
         ProcessQueryTicket_ChangesInterp(s, s', query_ticket);
+
+        assert s.tickets == s'.tickets + multiset{query_ticket};
+
+        if query_ticket.input.key in I(s).s.m {
+          assert B.LinearizationPoint(I(s), I(s'), query_ticket.rid, query_ticket.input,
+              MapIfc.QueryOutput(Found(I(s).s.m[query_ticket.input.key])));
+        } else {
+          assert B.LinearizationPoint(I(s), I(s'), query_ticket.rid, query_ticket.input,
+              MapIfc.QueryOutput(NotFound));
+        }
       }
     }
   }
+
+  lemma NewTicket_RefinesMap(s: A.Variables, s': A.Variables, rid: int, input: MapIfc.Input)
+    requires A.Inv(s)
+    requires A.NewTicket(s, s', rid, input)
+    ensures A.Inv(s')
+    ensures B.Next(I(s), I(s'), Ifc.Start(rid, input))
+  {
+    assert s'.table == s.table;
+    assert s'.stubs == s.stubs;
+    MultisetLemmas.MultisetSimplificationTriggers<HT.Ticket, B.Req>();
+    //assert s'.tickets == s.tickets + multiset{HT.Ticket(rid, input)};
+    //assert I(s').reqs == I(s).reqs + multiset{B.Req(rid, input)};
+    //assert I(s').s == I(s).s;
+  }
+
+  lemma ConsumeStub_RefinesMap(s: A.Variables, s': A.Variables, rid: int, output: MapIfc.Output)
+    requires A.Inv(s)
+    requires A.ConsumeStub(s, s', rid, output)
+    ensures A.Inv(s')
+    ensures B.Next(I(s), I(s'), Ifc.End(rid, output))
+  {
+    assert s'.table == s.table;
+    assert s'.tickets == s.tickets;
+    assert s.stubs == s'.stubs + multiset{HT.Stub(rid, output)};
+    MultisetLemmas.MultisetSimplificationTriggers<HT.Stub, B.Resp>();
+    /*assert s.stubs == s'.stubs + multiset{HT.Stub(rid, output)};
+    assert I(s).resps == I(s').resps + multiset{B.Resp(rid, output)};
+    assert I(s').resps == I(s).resps - multiset{B.Resp(rid, output)};
+    assert I(s').s == I(s).s;
+    assert I(s').reqs == I(s).reqs;
+    assert B.Resp(rid, output) in I(s).resps;*/
+  }
+
 }
